safe regions + following fix

abstract_machine.v
@@ -1,6 +1,6 @@
-Require Import Util.
-Require Import rewriting_system.
-Require Import Entropy.
+Require Import Util
+               Entropy.
+Require Export rewriting_system.
 
 
 
@@ -24,14 +24,6 @@ Module Type ABSTRACT_MACHINE.
   Instance rws : REWRITING_SYSTEM configuration :=
   { transition := transition }.
 
-(* Uncomment if you don't want to use classes:
-
-  Notation "c1 → c2"  := (transition c1 c2)              (no associativity, at level 70).
-  Notation "t1 →+ t2" := (clos_trans_1n _ transition t1 t2) 
-                                                         (no associativity, at level 70).
-  Notation "t1 →* t2" := (clos_refl_trans_1n _ transition t1 t2) 
-                                                         (no associativity, at level 70).
-*)
 
   Axioms
   (final_correct :                                                              forall c,
@@ -40,6 +32,16 @@ Module Type ABSTRACT_MACHINE.
        c1 → c2 <-> exists e, next_conf e c1 = Some c2)
   (finals_are_vals :                                                          forall c v,
        final c = Some v <-> c = v).
+
+
+
+  Class SafeRegion (P : configuration -> Prop) :=
+  { 
+      preservation :                                                        forall c1 c2,
+          P c1  ->  c1 → c2  ->  P c2;
+      progress :                                                               forall c1,
+          P c1  ->  (exists (v : value), c1 = v) \/ (exists c2, c1 → c2)
+  }.
 
 End ABSTRACT_MACHINE.
 
@@ -55,31 +57,3 @@ Module Type ABSTRACT_MACHINE_DET (AM : ABSTRACT_MACHINE).
 
 End ABSTRACT_MACHINE_DET.
 
-
-
-
-Module Type AM_SAFE_REGION (AM : ABSTRACT_MACHINE).
-
-  Import AM.
-
-  Parameter safe : configuration -> Prop.
-
-  Axioms
-  (preservation :                                                           forall c1 c2,
-       safe c1 -> c1 → c2 -> safe c2)
-  (progress :                                                                   forall c,
-       safe c -> (exists v, c = v) \/ (exists c', c → c')).
-
-End AM_SAFE_REGION.
-
-
-
-
-Module Type AM_PROGRESS (AM : ABSTRACT_MACHINE).
-
-  Import AM.
-
-  Axiom progress :                                                            forall t c,
-      (load t →* c) -> (exists v, c = v) \/ (exists c', c → c').
-
-End AM_PROGRESS.
